TabularTypeInterpreter/F⊗⊕ω/Lemmas/Value.lean
@@ -5,9 +5,10 @@ import TabularTypeInterpreter.«F⊗⊕ω».Lemmas.Type.ParallelReduction
 
 namespace TabularTypeInterpreter.«F⊗⊕ω»
 
-theorem TypeEquivalence.common_reduct_of (eq: [[Δ ⊢ A ≡ B]]) (wf: [[ ⊢ Δ ]]) (lc: A.TypeVarLocallyClosed) : ∃C, [[Δ ⊢ A <≡>* C]] ∧ [[Δ ⊢ B <≡>* C]] :=
-  eq.EqParallelReduction_of.common_reduct wf lc
-
+theorem TypeEquivalence.common_reduct_of (eq: [[Δ ⊢ A ≡ B]]) (wf: [[ ⊢ Δ ]]) (Alc: A.TypeVarLocallyClosed) : ∃C, [[Δ ⊢ A ≡>* C]] ∧ [[Δ ⊢ B ≡>* C]] :=
+  have ered := eq.EqParallelReduction_of
+  have Blc := ered.preserve_lc.1 Alc
+  ered.common_reduct wf Alc Blc
 namespace Value
 
 -- TODO rename, and will be affected by equiv definition change
